ChecksumLog.v: representation for a list of values and its hash program and correctness proof for Hash on a list of values

src/ChecksumLog.v
@@ -14,6 +14,7 @@ Require Import SepAuto.
 Require Import List.
 Require Import Array.
 Require Import EqdepFacts.
+Require Import Arith.
 
 Set Implicit Arguments.
 
@@ -23,19 +24,132 @@ Definition default_valu : valu := $0.
 Definition hash_block : addr := $2.
 
 
-Definition hash2 (a b : word valulen) := hash_to_valu (hash_fwd (Word.combine a b)).
+Definition hash2 sz1 sz2 (a : word sz1) (b : word sz2) :=
+  hash_fwd (Word.combine a b).
 
-Definition hash2_rep a b v :=
+Definition hash2_valu (a b : valu) :=
+  hash2 a (hash2 b default_valu).
+
+Definition hash2_rep sz1 sz2 (a : word sz1) (b : word sz2) v :=
   v = hash2 a b /\
-  hash_inv (hash_fwd (Word.combine a b)) = existT _ _ (Word.combine a b).
+  hash_inv v = existT _ _ (Word.combine a b).
 
+Inductive hash_list_rep : (list valu) -> word hashlen -> Prop :=
+  | HL_nil : forall hl,
+      hl = hash_fwd default_valu ->
+      hash_inv hl = existT _ _ default_valu ->
+        hash_list_rep nil hl
+  | HL_cons : forall values hvalues hvalues' x,
+      hash_list_rep values hvalues ->
+      hash2_rep x hvalues hvalues' ->
+      hash_list_rep (x :: values) hvalues'.
+
+
+(* Program that hashes a list of values into a single hash value. *)
+Definition hash_list T values rx : prog T :=
+    default_hash <- Hash default_valu;
+    let^ (hash) <- For i < $ (length values)
+    Ghost [ crash ]
+    Loopvar [ hash ]
+    Continuation lrx
+    Invariant
+      [[ hash_list_rep (rev (firstn #i values)) hash ]]
+    OnCrash crash
+    Begin
+      hash <- Hash (Word.combine (sel values i default_valu) hash);
+      lrx ^(hash)
+    Rof ^(default_hash);
+    rx hash.
+
+
+Theorem hash_list_ok : forall values,
+  {< (_ : unit) ,
+  PRE
+    emp * [[ goodSize addrlen (length values) ]]
+  POST RET:hash
+    emp * [[ hash_list_rep (rev values) hash ]]
+  CRASH
+    emp
+  >} hash_list values.
+Proof.
+  unfold hash_list.
+  step.
+  step.
+  constructor; auto.
+  step.
+  step.
+
+  assert (Hlength: length (rev (firstn # (m ^+ $ (1)) values)) = S (# (m))).
+    rewrite rev_length.
+    rewrite firstn_length.
+    erewrite wordToNat_plusone; eauto.
+    destruct (le_dec (S (# m)) (length values)).
+      apply Min.min_l. auto.
+
+      apply not_lt in n.
+      apply wlt_lt in H.
+      rewrite wordToNat_natToWord_idempotent' in H; auto.
+      intuition.
+
+  (* Loop invariant. *)
+  - destruct (rev (firstn # (m ^+ $ (1)) values)) eqn:Hrev_values.
+    + simpl in Hlength. inversion Hlength.
+    + eapply HL_cons.
+      assert (Hl: rev l = (firstn # (m) values)).
+        replace l with (rev (rev l)) in Hrev_values;
+          try apply rev_involutive.
+        rewrite <- rev_unit in Hrev_values.
+        erewrite wordToNat_plusone in Hrev_values; eauto.
+        apply rev_injective in Hrev_values.
+
+        rewrite <- removelast_firstn;
+          try (apply lt_word_lt_nat; auto).
+        replace (rev l) with (rev l ++ removelast (w :: nil)).
+        rewrite <- removelast_app.
+        rewrite Hrev_values.
+        auto.
+
+        intuition. inversion H3.
+        simpl. rewrite app_nil_r. auto.
+
+      rewrite <- rev_involutive in Hl.
+      apply rev_injective in Hl.
+      rewrite Hl. eauto.
+      unfold hash2_rep, hash2.
+      assert (Hw: selN (firstn # (m ^+ $ (1)) values) (# m) default_valu = w).
+        rewrite <- rev_involutive in Hrev_values.
+        apply rev_injective in Hrev_values.
+        rewrite Hrev_values.
+        simpl. apply selN_last. rewrite rev_length.
+        simpl in Hlength. apply eq_add_S in Hlength.
+        auto.
+      rewrite selN_firstn in Hw;
+        try (erewrite wordToNat_plusone; eauto).
+      subst.
+      intuition.
+
+  (* Loop invariant implies post-condition. *)
+  - step.
+    assert (Hfirstn: firstn # (natToWord addrlen (length values)) values = values).
+      rewrite wordToNat_natToWord_idempotent'; auto.
+      apply firstn_oob. auto.
+    rewrite <- Hfirstn. auto.
+
+  Grab Existential Variables.
+  all: eauto.
+Qed.
+
+Hint Extern 1 ({{_}} progseq (hash_list _ _ _) _) => apply hash_list_ok : prog.
+
+
+(* Representations for an example with two log blocks. *)
 (* block1 and block2 are synced, hash_block has some valid hash *)
-Definition any_hash_rep a b a' b' (d : @mem addr (@weq addrlen) valuset) :
+Definition any_hash_rep (a b a' b' : valu) (d : @mem addr (@weq addrlen) valuset) :
     @pred addr (@weq addrlen) valuset :=
   (exists hv,
     [[ (block1 |-> (a, nil) *
      block2 |-> (b, nil) *
-     hash_block |-> (hv, nil))%pred d ]] *
+     hash_block |-> (hash_to_valu hv, nil))%pred d ]] *
     [[ hash2_rep a' b' hv ]])%pred.
 
 (* hash_block has the valid hash of block1 and block2 values *)
@@ -49,21 +163,20 @@ Definition rep a b (d : @mem addr (@weq addrlen) valuset) :
     - hash of old values
     - hash of new values but unsynced
     - hash of new values and synced *)
-Definition crep a b a' b' :
+Definition crep (a b a' b' : valu) :
     @pred addr (@weq addrlen) valuset :=
   (exists hv hv',
     block1 |->? *
     block2 |->? *
-    ( hash_block |-> (hv, nil) *
+    ( hash_block |-> (hash_to_valu hv, nil) *
         [[ hash2_rep a b hv ]] \/
-      hash_block |-> (hv', hv :: nil) *
+      hash_block |-> (hash_to_valu hv', hash_to_valu hv :: nil) *
         [[ hash2_rep a b hv /\ hash2_rep a' b' hv' ]] \/
-      hash_block |-> (hv', nil) *
+      hash_block |-> (hash_to_valu hv', nil) *
         [[ hash2_rep a' b' hv' ]]))%pred.
 
 
 (* Example "log" implementation using checksums *)
-
 Definition put T cs d1 d2 rx : prog T :=
   cs <- BUFCACHE.write block1 d1 cs;
   cs <- BUFCACHE.write block2 d2 cs;
@@ -146,12 +259,12 @@ Proof.
 Qed.
 
 (* block1 and block2 get some value, and hash_block points to a valid hash of  *)
-Definition after_crash_pred v1 v2 :
+Definition after_crash_pred (v1 v2 : valu) :
     @pred addr (@weq addrlen) valuset :=
   (exists a b hv,
       block1 |-> (a, nil) *
       block2 |-> (b, nil) *
-      hash_block |-> (hv, nil) *
+      hash_block |-> (hash_to_valu hv, nil) *
     [[ hash2_rep v1 v2 hv ]])%pred.
 
 Lemma crash_xform_would_recover_either_pred : forall v1 v2 v1' v2',
@@ -212,14 +325,14 @@ Proof.
     destruct H5.
 
     assert (Hheq: d1_old = a /\ d2_old = b).
-      apply hash_to_valu_inj in H0.
-      rewrite H0 in H11.
+      subst.
+      apply hash_to_valu_inj in H8.
+      rewrite H8 in H3.
       rewrite H11 in H3.
       pose proof (eq_sigT_snd H3).
       autorewrite with core in *.
-      apply combine_inj in H5.
-      destruct H5.
-      auto.
+      apply combine_inj in H0.
+      intuition.
     unfold any_hash_rep, hash2_rep.
     cancel.
 
@@ -242,14 +355,14 @@ Proof.
     destruct H5.
 
     assert (Hheq: d1 = a /\ d2 = b).
-      apply hash_to_valu_inj in H0.
-      rewrite H0 in H11.
+      subst.
+      apply hash_to_valu_inj in H8.
+      rewrite H8 in H3.
       rewrite H11 in H3.
       pose proof (eq_sigT_snd H3).
       autorewrite with core in *.
-      apply combine_inj in H5.
-      destruct H5.
-      auto.
+      apply combine_inj in H0.
+      intuition.
     unfold any_hash_rep, hash2_rep.
     cancel.
 
